src/lemmas/inversion.lean
@@ -70,3 +70,55 @@ begin
   existsi et_τ1,
   exact et_a,
 end
+
+theorem inversion_sum_left
+  {Γ: cx typ} {e: exp} {τ2 τ: typ}
+  (et: has_typ Γ (exp.sum_left τ2 e) τ)
+  : ∃ (τ1: typ), τ = typ.sum τ1 τ2 ∧ has_typ Γ e τ1 :=
+begin
+  cases et,
+  existsi et_τ1,
+  split,
+  refl,
+  exact et_a,
+end
+
+theorem inversion_sum_right
+  {Γ: cx typ} {e: exp} {τ1 τ: typ}
+  (et: has_typ Γ (exp.sum_right τ1 e) τ)
+  : ∃ (τ2: typ), τ = typ.sum τ1 τ2 ∧ has_typ Γ e τ2 :=
+begin
+  cases et,
+  existsi et_τ2,
+  split,
+  refl,
+  exact et_a,
+end
+
+theorem inversion_case_never
+  {Γ: cx typ} {e: exp} {τ τ': typ}
+  (et: has_typ Γ (exp.case_never τ e) τ')
+  : τ = τ' ∧ has_typ Γ e typ.never :=
+begin
+  cases et,
+  split,
+  refl,
+  exact et_a,
+end
+
+theorem inversion_case
+  {Γ: cx typ} {eh e1 e2: exp} {x1 x2: var} {τ: typ}
+  (et: has_typ Γ (exp.case eh x1 e1 x2 e2) τ)
+  : ∃ (τ1 τ2: typ),
+    has_typ Γ eh (typ.sum τ1 τ2) ∧
+    has_typ (cx.insert Γ x1 τ1) e1 τ ∧
+    has_typ (cx.insert Γ x2 τ2) e2 τ :=
+begin
+  cases et,
+  existsi [et_τ1, et_τ2],
+  split,
+  exact et_a,
+  split,
+  exact et_a_1,
+  exact et_a_2,
+end
